src/program_proof/simplepb/config2_proof.v
@@ -1,0 +1,393 @@
+From Perennial.program_proof Require Import grove_prelude.
+From Goose.github_com.mit_pdos.gokv.simplepb Require Export config2.
+From iris.algebra Require Import dfrac_agree mono_list.
+From Perennial.program_proof Require Import marshal_stateless_proof std_proof.
+From Perennial.program_proof.simplepb Require Import config_marshal_proof renewable_lease.
+From Perennial.program_proof.grove_shared Require Import urpc_proof.
+From iris.base_logic Require Export lib.ghost_var mono_nat.
+From Perennial.program_proof.mpaxos Require Import tryacquire_proof.
+
+Section config_global.
+
+Record config_names :=
+{
+  epoch_gn:gname ;
+  repoch_gn:gname ;
+  config_val_gn:gname;
+}.
+
+Class configG Σ := {
+    config_configG :> ghost_varG Σ (list u64) ;
+    config_urpcG :> urpcregG Σ ;
+    config_epochG :> mono_natG Σ ;
+    config_mpG :> mpG Σ ;
+    config_leaseG :> renewable_leaseG Σ ;
+}.
+
+Definition configΣ := #[mono_natΣ ; ghost_varΣ (list u64) ; urpcregΣ ; renewable_leaseΣ ].
+
+Global Instance subG_configΣ {Σ} : subG configΣ Σ → configG Σ.
+Proof. intros. (* solve_inG. Qed. *)
+       Admitted. (* FIXME: mpΣ *)
+
+Implicit Type γ : config_names.
+
+Context `{!gooseGlobalGS Σ}.
+Context `{!configG Σ}.
+
+Definition own_latest_epoch γ (epoch:u64) : iProp Σ :=
+  mono_nat_auth_own γ.(epoch_gn) (1/2) (int.nat epoch).
+
+Definition own_reserved_epoch γ (epoch:u64) : iProp Σ :=
+  mono_nat_auth_own γ.(repoch_gn) (1/2) (int.nat epoch).
+
+Definition is_reserved_epoch_lb γ (epoch:u64) : iProp Σ :=
+  mono_nat_lb_own γ.(repoch_gn) (int.nat epoch).
+
+Definition own_config γ (conf:list u64) : iProp Σ :=
+  ghost_var γ.(config_val_gn) (1/2) conf
+.
+
+Definition epochLeaseN := nroot .@ "epochLeaseN".
+
+Program Definition ReserveEpochAndGetConfig_core_spec γ Φ :=
+  (
+    £ 1 -∗
+    (|={⊤,∅}=> ∃ reservedEpoch conf, own_reserved_epoch γ reservedEpoch ∗ own_config γ conf ∗
+    (⌜int.nat reservedEpoch < int.nat (word.add reservedEpoch (U64 1))⌝ -∗
+      own_reserved_epoch γ (word.add reservedEpoch (U64 1)) -∗ own_config γ conf ={∅,⊤}=∗
+      Φ (word.add reservedEpoch 1) conf
+      ))
+    )%I.
+
+Program Definition GetConfig_core_spec γ Φ :=
+  (£ 1 ={⊤,∅}=∗ ∃ conf, own_config γ conf ∗ (own_config γ conf ={∅,⊤}=∗ Φ conf))%I.
+
+Program Definition TryWriteConfig_core_spec γ (epoch:u64) (new_conf:list u64) Φ : iProp Σ :=
+  is_reserved_epoch_lb γ epoch ∗
+  (£ 1 -∗ |={⊤,↑epochLeaseN}=> ∃ latest_epoch reserved_epoch,
+   own_latest_epoch γ latest_epoch ∗
+   own_reserved_epoch γ reserved_epoch ∗
+   if (decide (reserved_epoch = epoch)) then
+     ∃ conf, own_config γ conf ∗
+                        (own_config γ new_conf -∗
+                         own_reserved_epoch γ reserved_epoch -∗
+                         own_latest_epoch γ epoch ={↑epochLeaseN,⊤}=∗ Φ (U64 0))
+      else
+        (own_latest_epoch γ latest_epoch -∗
+         own_reserved_epoch γ reserved_epoch
+         ={↑epochLeaseN,⊤}=∗ (∀ (err:u64), ⌜err ≠ 0⌝ → Φ err))
+  ).
+
+Program Definition GetLease_core_spec γ (epoch:u64) Φ : iProp Σ :=
+  (∀ (leaseExpiration:u64) γl,
+    is_lease epochLeaseN γl (own_latest_epoch γ epoch) -∗
+    is_lease_valid_lb γl leaseExpiration -∗ Φ (U64 0) leaseExpiration
+  ) ∧
+  (∀ (err:u64), ⌜err ≠ 0⌝ → Φ err (U64 0))
+.
+
+Program Definition ReserveEpochAndGetConfig_spec γ :=
+  λ (encoded_args:list u8), λne (Φ : list u8 -d> iPropO Σ) ,
+  ( (* no args *)
+    ReserveEpochAndGetConfig_core_spec γ (λ newEpoch conf,
+                                  ∀ enc_conf,
+                                   ⌜Config.has_encoding enc_conf conf⌝ -∗
+                                   Φ (u64_le 0 ++ u64_le newEpoch ++ enc_conf)
+                                  ) ∗
+    (∀ err, ⌜ err ≠ U64 0 ⌝ -∗ Φ (u64_le err))
+    )%I.
+Next Obligation.
+  rewrite /ReserveEpochAndGetConfig_core_spec.
+  solve_proper.
+Defined.
+
+Program Definition GetConfig_spec γ :=
+  λ (encoded_args:list u8), λne (Φ : list u8 -d> iPropO Σ) ,
+  ( (* no args *)
+    GetConfig_core_spec γ (λ conf, ∀ reply,
+                                   ⌜Config.has_encoding reply conf⌝ -∗
+                                   Φ reply
+                                  )
+    )%I.
+Next Obligation.
+  solve_proper.
+Defined.
+
+Program Definition TryWriteConfig_spec γ :=
+  λ (enc_args:list u8), λne (Φ : list u8 -d> iPropO Σ) ,
+  ( ∃ epoch new_conf enc_new_conf,
+    ⌜enc_args = u64_le epoch ++ enc_new_conf⌝ ∗
+    ⌜Config.has_encoding enc_new_conf new_conf⌝ ∗
+    TryWriteConfig_core_spec γ epoch new_conf (λ err, ∀ reply,
+                                   ⌜reply = u64_le err⌝ -∗
+                                   Φ reply
+                                  )
+    )%I.
+Next Obligation.
+  unfold TryWriteConfig_core_spec.
+  solve_proper.
+Defined.
+
+Program Definition GetLease_spec γ :=
+  λ (enc_args:list u8), λne (Φ : list u8 -d> iPropO Σ) ,
+  ( ∃ epoch ,
+    ⌜enc_args = u64_le epoch⌝ ∗
+    GetLease_core_spec γ epoch (λ (err:u64) (leaseExpiration:u64), ∀ reply,
+                                   ⌜reply = u64_le err ++ u64_le leaseExpiration⌝ -∗
+                                   Φ reply
+                                  )
+    )%I.
+Next Obligation.
+  unfold GetLease_core_spec.
+  solve_proper.
+Defined.
+
+Definition is_config_host (host:u64) γ : iProp Σ :=
+  ∃ γrpc,
+  is_urpc_spec_pred γrpc host (U64 0) (ReserveEpochAndGetConfig_spec γ) ∗
+  is_urpc_spec_pred γrpc host (U64 1) (GetConfig_spec γ) ∗
+  is_urpc_spec_pred γrpc host (U64 2) (TryWriteConfig_spec γ) ∗
+  is_urpc_spec_pred γrpc host (U64 3) (GetLease_spec γ) ∗
+  is_urpc_dom γrpc {[ (U64 0) ; (U64 1) ; (U64 2) ; (U64 3) ]}
+.
+
+End config_global.
+
+Module state.
+Section state.
+Record t :=
+  mk {
+      epoch : u64 ;
+      reservedEpoch : u64 ;
+      leaseExpiration : u64 ;
+      wantLeaseToExpire : bool ;
+      config : list u64 ;
+    }.
+
+Definition encode (x:t) : list u8.
+Admitted.
+
+Context `{!heapGS Σ}.
+Definition own (l:loc) (x:t) : iProp Σ.
+Admitted.
+
+End state.
+End state.
+
+Section config_proof.
+
+Context `{!heapGS Σ}.
+Context `{!configG Σ}.
+
+Definition is_Clerk (ck:loc) γ : iProp Σ :=
+  ∃ (cl:loc) srv,
+  "#Hcl" ∷ readonly (ck ↦[config.Clerk :: "cl"] #cl) ∗
+  "#Hcl_rpc"  ∷ is_uRPCClient cl srv ∗
+  "#Hhost" ∷ is_config_host srv γ
+.
+
+Lemma wp_MakeClerk configHost γ:
+  {{{
+      is_config_host configHost γ
+  }}}
+    config.MakeClerk #configHost
+  {{{
+      ck, RET #ck; is_Clerk ck γ
+  }}}
+.
+Proof.
+  iIntros (Φ) "#Hhost HΦ".
+  wp_call.
+  wp_apply (wp_MakeClient).
+  iIntros (cl) "#Hcl".
+  iApply wp_fupd.
+  wp_apply (wp_allocStruct).
+  { eauto. }
+  iIntros (ck) "Hck".
+  iDestruct (struct_fields_split with "Hck") as "HH".
+  iNamed "HH".
+  iMod (readonly_alloc_1 with "cl") as "#cl".
+  iModIntro.
+  iApply "HΦ".
+  iExists _, _. iFrame "#".
+Qed.
+
+Definition own_Config_ghost γ (st:state.t) : iProp Σ :=
+  "Hconf_ghost" ∷ own_config γ st.(state.config) ∗
+  "Hreserved_ghost" ∷ own_reserved_epoch γ st.(state.reservedEpoch) ∗
+  "Hepoch_lease" ∷ ((∃ γl, own_lease_expiration γl st.(state.leaseExpiration) ∗
+                          post_lease epochLeaseN γl (own_latest_epoch γ st.(state.epoch)))
+                   ) ∗
+   "%HresIneq" ∷ ⌜ int.nat st.(state.epoch) <= int.nat st.(state.reservedEpoch) ⌝
+.
+
+(*
+Lemma lease_expired_get_epoch γ leaseExpiration epoch :
+  is_time_lb leaseExpiration -∗
+  own_Config_ghost γ leaseExpiration epoch ={↑epochLeaseN}=∗
+  own_latest_epoch γ epoch
+.
+Proof.
+  iIntros "Htime_lb Hghost".
+  iDestruct "Hghost" as "[H | $]"; last done.
+  iDestruct "H" as (?) "(_ & Hexp & Hpost_lease)".
+  iMod (lease_expire with "Hexp Hpost_lease Htime_lb") as ">$"; done.
+Qed.
+
+Lemma lease_acc_epoch γ t leaseExpiration epoch :
+  own_time t -∗
+  own_Config_ghost γ leaseExpiration epoch ={↑epochLeaseN, ∅}=∗
+  own_latest_epoch γ epoch ∗ (own_latest_epoch γ epoch ={∅,↑epochLeaseN}=∗
+                       own_time t ∗
+                       own_Config_ghost γ leaseExpiration epoch
+                      ).
+Proof.
+  iIntros "Ht Hghost".
+  iDestruct "Hghost" as "[H | Hepoch]".
+  2:{ (* case: we own the epoch directly; just do some meaningless stuff to get
+         the right masks *)
+    iFrame "Hepoch".
+    iApply fupd_mask_intro.
+    { set_solver. }
+    iIntros "Hmask".
+    iIntros "Hepoch".
+    iMod "Hmask" as "_".
+    by iFrame.
+  }
+  {
+    iDestruct "H" as (?) "(#Hlease & Hexp & Hpost)".
+    destruct (decide (int.nat t < int.nat leaseExpiration)) eqn:Hineq.
+    { (* case: lease is unexpired. Access own_latest_epoch from the lease. *)
+      iDestruct (lease_get_lb with "Hexp") as "#Hvalid".
+      iMod (lease_acc with "Hvalid Hlease Ht") as "[>$ HH]".
+      { done. }
+      { done. }
+      replace (↑epochLeaseN ∖ ↑epochLeaseN) with (∅:coPset) by set_solver.
+      iModIntro.
+      iIntros "Hepoch".
+      iMod ("HH" with "Hepoch") as "$".
+      iModIntro.
+      iLeft.
+      iExists _; iFrame "∗#".
+    }
+    { (* case: lease is expired.  *)
+      iDestruct (own_time_get_lb with "Ht") as "#Hlb".
+      iMod (lease_expire with "Hexp Hpost [Hlb]") as ">Hepoch".
+      { iApply is_time_lb_mono; last done. word. }
+      iApply fupd_mask_intro.
+      { set_solver. }
+      iIntros "Hmask".
+      iFrame.
+      iIntros "Hepoch".
+      iMod "Hmask". iModIntro.
+      iFrame.
+    }
+  }
+Qed. *)
+
+Context `{config:list mp_server_names}.
+Context `{Pwf:state.t → iProp Σ}.
+Context {N:namespace}.
+
+Definition configWf (a:list u8) : iProp Σ :=
+  ∃ st, ⌜ a = state.encode st ⌝ ∗ Pwf st
+.
+
+Instance c : mpaxosParams.t Σ :=
+  mpaxosParams.mk Σ config configWf N
+.
+
+Definition is_config_inv γ γst : iProp Σ :=
+  inv N (∃ st,
+        "Hst" ∷ own_state γst (state.encode st) ∗
+        "Hghost" ∷ own_Config_ghost γ st
+      )
+.
+
+Definition own_Server (s:loc) γ : iProp Σ :=
+  ∃ (p:loc) γp γsrv γst,
+  "Hs" ∷ s ↦[config.Server :: "p"] #p ∗
+  "#Hsrv" ∷ is_Server p γp γsrv ∗
+  "#Hst_inv" ∷ is_state_inv γst γp ∗
+  "#Hconfig_inv" ∷ is_config_inv γ γst
+.
+
+Definition configN := nroot .@ "config".
+
+Definition is_Server (s:loc) γ : iProp Σ :=
+  ∃ mu,
+  "#Hmu" ∷ readonly (s ↦[config.Server :: "mu"] mu) ∗
+  "#His_mu" ∷ is_lock configN mu (own_Server s γ).
+
+Definition own_tryRelease (f:val) γ (st_ptr:loc) (oldst:state.t) : iProp Σ :=
+  ∀ (newst:state.t) Φ,
+  (
+    "Hvol" ∷ state.own st_ptr newst ∗
+    "Hwf" ∷ □ Pwf newst ∗
+    "Hupd" ∷ (own_Config_ghost γ oldst ={⊤∖↑N}=∗ own_Config_ghost γ newst ∗ Φ #true)
+  ) -∗
+  (Φ #false) -∗
+  WP f #() {{ Φ }}
+.
+
+Lemma wp_Server__tryAcquire s γ :
+  {{{
+        is_Server s γ
+  }}}
+    config2.Server__tryAcquire #s
+  {{{
+        (ok:bool) (st_ptr:loc) (f:val), RET (#ok, #st_ptr, f);
+        if ok then
+          ∃ st,
+          state.own st_ptr st ∗
+          own_tryRelease f γ st_ptr st
+        else
+          True
+  }}}
+.
+Proof.
+Admitted.
+
+Lemma wp_Server__ReserveEpochAndGetConfig (server:loc) γ :
+  {{{
+        is_Server server γ
+  }}}
+    config2.Server__ReserveEpochAndGetConfig #server
+  {{{
+        (f:val), RET f; is_urpc_handler_pred f (ReserveEpochAndGetConfig_spec γ)
+  }}}.
+Proof.
+  iIntros (Φ) "#His_srv HΦ".
+  wp_call.
+  iApply "HΦ".
+  iModIntro.
+  unfold is_urpc_handler_pred.
+  clear Φ.
+  iIntros (enc_args Ψ req_sl rep_ptr) "!# %Φ (Harg_sl & Hrep & HΨ) HΦ".
+  wp_call.
+
+  replace (slice.nil) with (slice_val Slice.nil) by done.
+  wp_apply (wp_WriteInt with "[]").
+  { iApply own_slice_zero. }
+  iIntros (rep_sl) "Hrep_sl".
+  wp_store.
+  wp_apply (wp_Server__tryAcquire with "[$]").
+  iIntros (???) "Hpost".
+  wp_pure1_credit "Hlc".
+  wp_if_destruct.
+  { (* if not ok from tryAcquire *)
+    iApply "HΦ".
+    iDestruct (own_slice_to_small with "Hrep_sl") as "$".
+    iFrame.
+    Opaque u64_le.
+    rewrite /ReserveEpochAndGetConfig_spec /ReserveEpochAndGetConfig_core_spec /=.
+    iRight in "HΨ".
+    iApply "HΨ".
+    done.
+  }
+  iDestruct "Hpost" as (?) "[Hvol Hwp]".
+  iNamed "Hvol".
+Admitted.
+
+End config_proof.
